etc.lean
@@ -22,13 +22,63 @@ lemma lt_of_add {n m: ℕ}: n < n + m + 1 ∧ m < n + m + 1 :=
   have h₂: m < n + m + 1, from lt_add_of_le_of_pos this zero_lt_one,
   ⟨h₁, h₂⟩
 
--- other auxiliary lemmas
+-- auxiliary lemmas for option
 
 lemma some.inj.inv {α: Type} {a b: α}: a = b → (some a = some b) :=
   assume : a = b,
-  by simp *
+  by simp [this]
 
-lemma is_none.inv {α: Type} (a: option α): option.is_none a ↔ (a = none) :=
+lemma option.some_iff_not_none {α: Type} {a: option α}: option.is_some a ↔ ¬ option.is_none a :=
+  begin
+    cases a,
+    split,
+    intro h,
+    contradiction,
+    intro h2,
+    unfold option.is_none at h2,
+    have h3: ↑tt = false, from eq_false_intro h2,
+    have h4: ↑tt = true, by simp,
+    have h5: false = true, from eq.trans h3.symm h4,
+    have h6: true, from trivial,
+    have h7: false, from h5.symm ▸ h6,
+    contradiction,
+    split,
+    intro h8,
+    intro h9,
+    contradiction,
+    intro h10,
+    unfold option.is_some,
+    change tt = tt,
+    refl
+  end
+
+lemma option.none_iff_not_some {α: Type} {a: option α}: option.is_none a ↔ ¬ option.is_some a :=
+  begin
+    cases a,
+    split,
+    intro h,
+    contradiction,
+    intro h2,
+    unfold option.is_none,
+    change tt = tt,
+    refl,
+    split,
+    intro h3,
+    intro h4,
+    unfold option.is_none at h3,
+    change ff = tt at h3,
+    contradiction,
+    intro h5,
+    unfold option.is_some at h5,
+    have h6: ↑tt = false, from eq_false_intro h5,
+    have h7: ↑tt = true, by simp,
+    have h8: false = true, from eq.trans h6.symm h7,
+    have h9: true, from trivial,
+    have : false, from h8.symm ▸ h9,
+    contradiction
+  end
+
+lemma option.is_none.inv {α: Type} {a: option α}: (a = none) ↔ option.is_none a :=
   begin
     cases a,
     case option.some v {
@@ -47,51 +97,48 @@ lemma is_none.inv {α: Type} (a: option α): option.is_none a ↔ (a = none) :=
     }
   end
 
-lemma not_is_none.inv {α: Type} (a: option α): ¬ option.is_none a → (a ≠ none) :=
-  assume is_not_none: ¬ option.is_none a,
-  begin
+lemma option.is_none.ninv {α: Type} {a: option α}: (a ≠ none) ↔ ¬ option.is_none a :=
+  by begin
+    split,
+    intro h,
     cases a,
-    case option.some v {
-      assume is_none_some,
-      contradiction
-    },
-    case option.none {
-      assume is_none_none,
-      have : (option.is_none none = tt), by unfold option.is_none,
-      contradiction
-    }
+    contradiction,
+    unfold option.is_none,
+    intro h2,
+    change ff = tt at h2,
+    contradiction,
+    intro h3,
+    intro h4,
+    rw[h4] at h3,
+    unfold option.is_none at h3,
+    have h5: ↑tt = false, from eq_false_intro h3,
+    have h6: ↑tt = true, by simp,
+    have h7: false = true, from eq.trans h5.symm h6,
+    have h8: true, from trivial,
+    have r9: false, from h7.symm ▸ h8,
+    contradiction
   end
 
-lemma exists_of_is_some {α: Type} {a: option α}: option.is_some a → (∃b, a = some b) :=
-  assume h: option.is_some a,
-  begin
-    cases a,
-    case option.none { contradiction },
-    case option.some b { exact exists.intro b rfl }
-  end
-
-lemma not_is_none.rinv {α: Type} {a: option α}: (∃b, a = some b) ↔ ¬ option.is_none a :=
+lemma option.is_some_iff_exists {α: Type} {a: option α}: option.is_some a ↔ (∃b, a = some b) :=
   begin
     split,
     cases a,
     assume c,
     cases c,
-    contradiction,
-    assume _,
-    unfold option.is_none,
-    apply ff_eq_tt_eq_false,
-    assume _,
-    cases a,
-    case option.some v {
-      exact exists.intro v rfl
-    },
-    case option.none {
-      have : (option.is_none none = tt), by unfold option.is_none,
-      contradiction
-    }
+    intro h,
+    existsi a,
+    refl,
+    intro h2,
+    cases h2,
+    rw[a_2],
+    unfold option.is_some,
+    change tt = tt,
+    refl
   end
 
-lemma mem_of_2set {α: Type} {a b c: α}:
+-- auxiliary lemmas for sets
+
+lemma set.two_elems_mem {α: Type} {a b c: α}:
   a ∈ ({b, c}: set α) -> (a = b) ∨ (a = c) :=
   assume a_in_bc: a ∈ {b, c},
   have a_in_bc: a ∈ insert b (insert c (∅: set α)), by { simp at a_in_bc, simp[a_in_bc] },
