freevars.lean
@@ -150,6 +150,23 @@ lemma free_in_prop.pre.inv {t₁ t₂: term} {x: var}:
     case free_in_prop.pre₂ free_in_t₂ { from or.inr free_in_t₂ } 
   end
 
+lemma free_in_prop.pre₁.inv {t: term} {op: unop} {x: var}:
+      free_in_prop x (prop.pre₁ op t) → free_in_term x t :=
+  assume x_free_in_pre: free_in_prop x (prop.pre₁ op t),
+  begin
+    cases x_free_in_pre,
+    case free_in_prop.preop free_in_t { from free_in_t }
+  end
+
+lemma free_in_prop.pre₂.inv {t₁ t₂: term} {op: binop} {x: var}:
+      free_in_prop x (prop.pre₂ op t₁ t₂) → free_in_term x t₁ ∨ free_in_term x t₂ :=
+  assume x_free_in_pre: free_in_prop x (prop.pre₂ op t₁ t₂),
+  begin
+    cases x_free_in_pre,
+    case free_in_prop.preop₁ free_in_t₁ { from or.inl free_in_t₁ },
+    case free_in_prop.preop₂ free_in_t₂ { from or.inr free_in_t₂ } 
+  end
+
 lemma free_in_prop.post.inv {t₁ t₂: term} {x: var}:
       free_in_prop x (prop.post t₁ t₂) → free_in_term x t₁ ∨ free_in_term x t₂ :=
   assume x_free_in_post: free_in_prop x (prop.post t₁ t₂),
@@ -157,6 +174,15 @@ lemma free_in_prop.post.inv {t₁ t₂: term} {x: var}:
     cases x_free_in_post,
     case free_in_prop.post₁ free_in_t₁ { from or.inl free_in_t₁ },
     case free_in_prop.post₂ free_in_t₂ { from or.inr free_in_t₂ } 
+  end
+
+lemma free_in_prop.call.inv {t₁ t₂: term} {x: var}:
+      free_in_prop x (prop.call t₁ t₂) → free_in_term x t₁ ∨ free_in_term x t₂ :=
+  assume x_free_in_call: free_in_prop x (prop.call t₁ t₂),
+  begin
+    cases x_free_in_call,
+    case free_in_prop.call₁ free_in_t₁ { from or.inl free_in_t₁ },
+    case free_in_prop.call₂ free_in_t₂ { from or.inr free_in_t₂ } 
   end
 
 lemma free_in_prop.forallc.inv {P: prop} {t: term} {x fx: var}:
@@ -172,6 +198,16 @@ lemma free_in_prop.forallc.inv {P: prop} {t: term} {x fx: var}:
     }
   end
 
+lemma free_in_prop.exis.inv {P: prop} {x fx: var}:
+      free_in_prop x (prop.exis fx P) → (x ≠ fx) ∧ (free_in_prop x P) :=
+  assume x_free_in_exis: free_in_prop x (prop.exis fx P),
+  begin
+    cases x_free_in_exis,
+    case free_in_prop.exis x_neq_fx free_in_P {
+      from ⟨x_neq_fx, free_in_P⟩ 
+    }
+  end
+
 lemma free_in_prop.implies.inv {P₁ P₂: prop} {x: var}: free_in_prop x (prop.implies P₁ P₂) → free_in_prop x P₁ ∨ free_in_prop x P₂ :=
   assume x_free_in_implies: free_in_prop x (prop.or P₁.not P₂),
   begin
@@ -184,6 +220,88 @@ lemma free_in_prop.implies.inv {P₁ P₂: prop} {x: var}: free_in_prop x (prop.
     },
     case free_in_prop.or₂ free_in_P₂ {
       show free_in_prop x P₁ ∨ free_in_prop x P₂, from or.inr free_in_P₂
+    }
+  end
+
+lemma free_in_prop.func.inv {P₁ P₂: prop} {t: term} {x y: var}:
+      free_in_prop x (prop.func t y P₁ P₂) → free_in_term x t ∨ (x ≠ y ∧ (free_in_prop x P₁ ∨ free_in_prop x P₂)) :=
+  assume : free_in_prop x (prop.func t y P₁ P₂),
+  have free_in_prop x (term.unop unop.isFunc t &&
+                      (prop.forallc y t (prop.implies P₁ (prop.pre t y)
+                                      && prop.implies (prop.post t y) P₂))), from this,
+  begin
+    cases this,
+    case free_in_prop.and₁ x_free_in_unopfunc {
+      cases x_free_in_unopfunc,
+      case free_in_prop.term x_free_in_unopfuncterm {
+        cases x_free_in_unopfuncterm,
+        case free_in_term.unop x_free_in_func {
+          left,
+          from x_free_in_func
+        }
+      }
+    },
+    case free_in_prop.and₂ x_free_in_forallc {
+      cases x_free_in_forallc,
+      case free_in_prop.forallc₁ x_neq_y x_free_in_t {
+        left,
+        from x_free_in_t
+      },
+      case free_in_prop.forallc₂ x_neq_y x_free_in_forallp {
+        cases x_free_in_forallp,
+        case free_in_prop.and₁ x_free_Rpre {
+          cases x_free_Rpre,
+          case free_in_prop.or₁ x_free_in_Pnot {
+            cases x_free_in_Pnot,
+            case free_in_prop.not x_free_in_P₁ {
+              right,
+              split,
+              from x_neq_y,
+              left,
+              from x_free_in_P₁
+            }
+          },
+          case free_in_prop.or₂ x_free_in_pre {
+            cases x_free_in_pre,
+            case free_in_prop.pre₁ x_free_in_t {
+              left,
+              from x_free_in_t
+            },
+            case free_in_prop.pre₂ x_free_in_y {
+              cases x_free_in_y,
+              case free_in_term.var {
+                contradiction
+              }
+            }
+          }
+        },
+        case free_in_prop.and₂ x_free_postS {
+          cases x_free_postS,
+          case free_in_prop.or₁ x_free_in_postnot {
+            cases x_free_in_postnot,
+            case free_in_prop.not x_free_in_post {
+              cases x_free_in_post,
+              case free_in_prop.post₁ x_free_in_t {
+                left,
+                from x_free_in_t
+              },
+              case free_in_prop.post₂ x_free_in_y {
+                cases x_free_in_y,
+                case free_in_term.var {
+                  contradiction
+                }
+              }
+            }
+          },
+          case free_in_prop.or₂ x_free_in_S {
+            right,
+            split,
+            from x_neq_y,
+            right,
+            from x_free_in_S
+          }
+        }
+      }
     }
   end
 
@@ -413,7 +531,7 @@ begin
         have : x ∉ σ', from ih.left.mp h4,
         have h5: ¬ (x = y), by begin
           by_contradiction,
-          have h6: (option.is_none (σ'.apply x) = tt), from (is_none.inv (σ'.apply x)).mpr h4,
+          have h6: (option.is_none (σ'.apply x) = tt), from option.is_none.inv.mp h4,
           have : (y = x ∧ option.is_none (σ'.apply x)), from ⟨a.symm, h6⟩,
           have : ((if y = x ∧ option.is_none (σ'.apply x) then ↑v' else σ'.apply x) = ↑v'),
           by simp[this],
@@ -482,7 +600,8 @@ begin
               have : (x = x ∧ option.is_none (σ'.apply x)), from ⟨rfl, h18⟩,
               exact h this
             end,
-            have : ∃v, (σ'.apply x) = some v, from not_is_none.rinv.mpr h19,
+            have : ((option.is_some (σ'.apply x)):Prop), from option.some_iff_not_none.mpr h19,
+            have : ∃v, (σ'.apply x) = some v, from option.is_some_iff_exists.mp this,
             cases this with v h20,
             have : ((if x = x ∧ option.is_none (σ'.apply x) then ↑v' else σ'.apply x) = σ'.apply x),
             by { simp[h], simp[h19] },
@@ -492,7 +611,8 @@ begin
         case env.contains.rest h27 {
           have : (∃v, σ'.apply x = some v), from ih.right.mpr h27,
           cases this with v h28,
-          have : ¬ (option.is_none (σ'.apply x)), from not_is_none.rinv.mp (exists.intro v h28),
+          have : ¬ (option.is_none (σ'.apply x)),
+          from option.some_iff_not_none.mp (option.is_some_iff_exists.mpr (exists.intro v h28)),
           have : ((if y = x ∧ option.is_none (σ'.apply x) then ↑v' else σ'.apply x) = σ'.apply x),
           by simp[this],
           show (∃v, (σ'[y↦v']) x = some v), from exists.intro v (eq.trans (eq.trans h17 this) h28)
@@ -501,3 +621,270 @@ begin
     end
   end
 end
+
+lemma free_in_termctx.binop.inv {x: var} {op: binop} {t₁ t₂: termctx} {t': term}:
+      x ∈ FV ((termctx.binop op t₁ t₂) t') → x ∈ FV (t₁ t') ∨ x ∈ FV (t₂ t') :=
+  assume x_free_in_t: x ∈ FV ((termctx.binop op t₁ t₂) t'),
+  have (termctx.apply (termctx.binop op t₁ t₂) t') = term.binop op (t₁.apply t') (t₂.apply t'),
+  by unfold termctx.apply,
+  have x ∈ FV (term.binop op (t₁.apply t') (t₂.apply t')), from this ▸ x_free_in_t,
+  show x ∈ FV (t₁ t') ∨ x ∈ FV (t₂ t'), from free_in_term.binop.inv this
+
+lemma free_in_termctx.term.inv {x: var} {t t': term}:
+      x ∈ FV (t.to_termctx t') → x ∈ FV t :=
+  assume x_free_in_t: x ∈ FV (t.to_termctx t'),
+  begin
+    induction t with v y unop t₁ ih₁ binop t₂ t₃ ih₂ ih₃ t₄ t₅ ih₄ ih₅,
+
+    show x ∈ FV (term.value v), from (
+      have term.to_termctx (term.value v) = (termctx.value v), by unfold term.to_termctx,
+      have h: x ∈ FV ((termctx.value v) t'), from this ▸ x_free_in_t,
+      have termctx.apply (termctx.value v) t' = (term.value v), by unfold termctx.apply,
+      show x ∈ FV (term.value v), from this.symm ▸ h
+    ),
+
+    show x ∈ FV (term.var y), from (
+      have term.to_termctx (term.var y) = termctx.var y, by unfold term.to_termctx,
+      have h: x ∈ FV ((termctx.var y) t'), from this ▸ x_free_in_t,
+      have termctx.apply (termctx.var y) t' = term.var y, by unfold termctx.apply,
+      show x ∈ FV (term.var y), from this.symm ▸ h
+    ),
+
+    show x ∈ FV (term.unop unop t₁), from (
+      have term.to_termctx (term.unop unop t₁) = termctx.unop unop t₁.to_termctx, by unfold term.to_termctx,
+      have h: x ∈ FV ((termctx.unop unop t₁.to_termctx) t'), from this ▸ x_free_in_t,
+      have termctx.apply (termctx.unop unop t₁.to_termctx) t' = term.unop unop (t₁.to_termctx.apply t'),
+      by unfold termctx.apply,
+      have x ∈ FV (term.unop unop (t₁.to_termctx.apply t')), from this ▸ h,
+      have x ∈ FV (t₁.to_termctx.apply t'), from free_in_term.unop.inv this,
+      have x ∈ FV t₁, from ih₁ this,
+      show x ∈ FV (term.unop unop t₁), from free_in_term.unop this
+    ),
+
+    show x ∈ FV (term.binop binop t₂ t₃), from (
+      have term.to_termctx (term.binop binop t₂ t₃) = termctx.binop binop t₂.to_termctx t₃.to_termctx,
+      by unfold term.to_termctx,
+      have h: x ∈ FV ((termctx.binop binop t₂.to_termctx t₃.to_termctx) t'), from this ▸ x_free_in_t,
+      have termctx.apply (termctx.binop binop t₂.to_termctx t₃.to_termctx) t'
+         = term.binop binop (t₂.to_termctx.apply t') (t₃.to_termctx.apply t'),
+      by unfold termctx.apply,
+      have x ∈ FV (term.binop binop (t₂.to_termctx.apply t') (t₃.to_termctx.apply t')), from this ▸ h,
+      have x ∈ FV (t₂.to_termctx.apply t') ∨ x ∈ FV (t₃.to_termctx.apply t'), from free_in_term.binop.inv this,
+      or.elim this (
+        assume : x ∈ FV (t₂.to_termctx.apply t'),
+        have x ∈ FV t₂, from ih₂ this,
+        show x ∈ FV (term.binop binop t₂ t₃), from free_in_term.binop₁ this
+      ) (
+        assume : x ∈ FV (t₃.to_termctx.apply t'),
+        have x ∈ FV t₃, from ih₃ this,
+        show x ∈ FV (term.binop binop t₂ t₃), from free_in_term.binop₂ this
+      )
+    ),
+
+    show x ∈ FV (term.app t₄ t₅), from (
+      have term.to_termctx (term.app t₄ t₅) = termctx.app t₄.to_termctx t₅.to_termctx,
+      by unfold term.to_termctx,
+      have h: x ∈ FV ((termctx.app t₄.to_termctx t₅.to_termctx) t'), from this ▸ x_free_in_t,
+      have termctx.apply (termctx.app t₄.to_termctx t₅.to_termctx) t'
+         = term.app (t₄.to_termctx.apply t') (t₅.to_termctx.apply t'),
+      by unfold termctx.apply,
+      have x ∈ FV (term.app (t₄.to_termctx.apply t') (t₅.to_termctx.apply t')), from this ▸ h,
+      have x ∈ FV (t₄.to_termctx.apply t') ∨ x ∈ FV (t₅.to_termctx.apply t'), from free_in_term.app.inv this,
+      or.elim this (
+        assume : x ∈ FV (t₄.to_termctx.apply t'),
+        have x ∈ FV t₄, from ih₄ this,
+        show x ∈ FV (term.app t₄ t₅), from free_in_term.app₁ this
+      ) (
+        assume : x ∈ FV (t₅.to_termctx.apply t'),
+        have x ∈ FV t₅, from ih₅ this,
+        show x ∈ FV (term.app t₄ t₅), from free_in_term.app₂ this
+      )
+    )
+  end
+
+lemma free_in_propctx.prop.inv {x: var} {P: prop} {t': term}:
+      x ∈ FV (P.to_propctx t') → x ∈ FV P :=
+  assume x_free_in_P: x ∈ FV (P.to_propctx t'),
+  begin
+    induction P,
+    case prop.term t { from (
+      have prop.to_propctx (prop.term t) = (propctx.term t), by unfold prop.to_propctx,
+      have h: x ∈ FV ((propctx.term t) t'), from this ▸ x_free_in_P,
+      have propctx.apply (propctx.term t.to_termctx) t' = t.to_termctx t', by unfold propctx.apply,
+      have x ∈ FV (prop.term (t.to_termctx t')), from this.symm ▸ h,
+      have x ∈ FV (t.to_termctx t'), from free_in_prop.term.inv this,
+      have x ∈ FV t, from free_in_termctx.term.inv this,
+      show x ∈ FV (prop.term t), from free_in_prop.term this
+    )},
+    case prop.not P₁ ih { from (
+      have prop.to_propctx (prop.not P₁) = (propctx.not P₁.to_propctx), by unfold prop.to_propctx,
+      have h: x ∈ FV ((propctx.not P₁.to_propctx) t'), from this ▸ x_free_in_P,
+      have propctx.apply (propctx.not P₁.to_propctx) t' = prop.not (P₁.to_propctx.apply t'), by unfold propctx.apply,
+      have x ∈ FV (prop.not (P₁.to_propctx.apply t')), from this.symm ▸ h,
+      have x ∈ FV (P₁.to_propctx.apply t'), from free_in_prop.not.inv this,
+      have x ∈ FV P₁, from ih this,
+      show x ∈ FV P₁.not, from free_in_prop.not this
+    )},
+    case prop.and P₁ P₂ ih₁ ih₂ { from (
+      have prop.to_propctx (prop.and P₁ P₂) = (P₁.to_propctx && P₂.to_propctx), by unfold prop.to_propctx,
+      have h: x ∈ FV ((P₁.to_propctx && P₂.to_propctx) t'), from this ▸ x_free_in_P,
+      have propctx.apply (propctx.and P₁.to_propctx P₂.to_propctx) t'
+         = (P₁.to_propctx.apply t') && (P₂.to_propctx.apply t'), by unfold propctx.apply,
+      have x ∈ FV ((P₁.to_propctx.apply t') && (P₂.to_propctx.apply t')), from this.symm ▸ h,
+      have x ∈ FV (P₁.to_propctx.apply t') ∨ x ∈ FV (P₂.to_propctx.apply t'), from free_in_prop.and.inv this,
+      or.elim this (
+        assume : x ∈ FV (P₁.to_propctx.apply t'),
+        have x ∈ FV P₁, from ih₁ this,
+        show x ∈ FV (P₁ && P₂), from free_in_prop.and₁ this
+      ) (
+        assume : x ∈ FV (P₂.to_propctx.apply t'),
+        have x ∈ FV P₂, from ih₂ this,
+        show x ∈ FV (P₁ && P₂), from free_in_prop.and₂ this
+      )
+    )},
+    case prop.or P₁ P₂ ih₁ ih₂ { from (
+      have prop.to_propctx (prop.or P₁ P₂) = (P₁.to_propctx || P₂.to_propctx), by unfold prop.to_propctx,
+      have h: x ∈ FV ((P₁.to_propctx || P₂.to_propctx) t'), from this ▸ x_free_in_P,
+      have propctx.apply (propctx.or P₁.to_propctx P₂.to_propctx) t'
+         = (P₁.to_propctx.apply t') || (P₂.to_propctx.apply t'), by unfold propctx.apply,
+      have x ∈ FV ((P₁.to_propctx.apply t') || (P₂.to_propctx.apply t')), from this.symm ▸ h,
+      have x ∈ FV (P₁.to_propctx.apply t') ∨ x ∈ FV (P₂.to_propctx.apply t'), from free_in_prop.or.inv this,
+      or.elim this (
+        assume : x ∈ FV (P₁.to_propctx.apply t'),
+        have x ∈ FV P₁, from ih₁ this,
+        show x ∈ FV (P₁ || P₂), from free_in_prop.or₁ this
+      ) (
+        assume : x ∈ FV (P₂.to_propctx.apply t'),
+        have x ∈ FV P₂, from ih₂ this,
+        show x ∈ FV (P₁ || P₂), from free_in_prop.or₂ this
+      )
+    )},
+    case prop.pre t₁ t₂ { from (
+      have prop.to_propctx (prop.pre t₁ t₂) = propctx.pre t₁ t₂, by unfold prop.to_propctx,
+      have h: x ∈ FV ((propctx.pre t₁ t₂) t'), from this ▸ x_free_in_P,
+      have propctx.apply (propctx.pre t₁.to_termctx t₂.to_termctx) t' = prop.pre (t₁.to_termctx t') (t₂.to_termctx t'),
+      by unfold propctx.apply,
+      have x ∈ FV (prop.pre (t₁.to_termctx t') (t₂.to_termctx t')), from this.symm ▸ h,
+      have x ∈ FV (t₁.to_termctx t') ∨ x ∈ FV (t₂.to_termctx t'), from free_in_prop.pre.inv this,
+      or.elim this (
+        assume : x ∈ FV (t₁.to_termctx t'),
+        have x ∈ FV t₁, from free_in_termctx.term.inv this,
+        show x ∈ FV (prop.pre t₁ t₂), from free_in_prop.pre₁ this
+      ) (
+        assume : x ∈ FV (t₂.to_termctx t'),
+        have x ∈ FV t₂, from free_in_termctx.term.inv this,
+        show x ∈ FV (prop.pre t₁ t₂), from free_in_prop.pre₂ this
+      )
+    )},
+    case prop.pre₁ op t { from (
+      have prop.to_propctx (prop.pre₁ op t) = propctx.pre₁ op t, by unfold prop.to_propctx,
+      have h: x ∈ FV ((propctx.pre₁ op t) t'), from this ▸ x_free_in_P,
+      have propctx.apply (propctx.pre₁ op t.to_termctx) t' = prop.pre₁ op (t.to_termctx t'),
+      by unfold propctx.apply,
+      have x ∈ FV (prop.pre₁ op (t.to_termctx t')), from this.symm ▸ h,
+      have x ∈ FV (t.to_termctx t'), from free_in_prop.pre₁.inv this,
+      have x ∈ FV t, from free_in_termctx.term.inv this,
+      show x ∈ FV (prop.pre₁ op t), from free_in_prop.preop this
+    )},
+    case prop.pre₂ op t₁ t₂ { from (
+      have prop.to_propctx (prop.pre₂ op t₁ t₂) = propctx.pre₂ op t₁ t₂, by unfold prop.to_propctx,
+      have h: x ∈ FV ((propctx.pre₂ op t₁ t₂) t'), from this ▸ x_free_in_P,
+      have propctx.apply (propctx.pre₂ op t₁.to_termctx t₂.to_termctx) t'
+         = prop.pre₂ op (t₁.to_termctx t') (t₂.to_termctx t'),
+      by unfold propctx.apply,
+      have x ∈ FV (prop.pre₂ op (t₁.to_termctx t') (t₂.to_termctx t')), from this.symm ▸ h,
+      have x ∈ FV (t₁.to_termctx t') ∨ x ∈ FV (t₂.to_termctx t'), from free_in_prop.pre₂.inv this,
+      or.elim this (
+        assume : x ∈ FV (t₁.to_termctx t'),
+        have x ∈ FV t₁, from free_in_termctx.term.inv this,
+        show x ∈ FV (prop.pre₂ op t₁ t₂), from free_in_prop.preop₁ this
+      ) (
+        assume : x ∈ FV (t₂.to_termctx t'),
+        have x ∈ FV t₂, from free_in_termctx.term.inv this,
+        show x ∈ FV (prop.pre₂ op t₁ t₂), from free_in_prop.preop₂ this
+      )
+    )},
+    case prop.post t₁ t₂ { from (
+      have prop.to_propctx (prop.post t₁ t₂) = propctx.post t₁ t₂, by unfold prop.to_propctx,
+      have h: x ∈ FV ((propctx.post t₁ t₂) t'), from this ▸ x_free_in_P,
+      have propctx.apply (propctx.post t₁.to_termctx t₂.to_termctx) t' = prop.post (t₁.to_termctx t') (t₂.to_termctx t'),
+      by unfold propctx.apply,
+      have x ∈ FV (prop.post (t₁.to_termctx t') (t₂.to_termctx t')), from this.symm ▸ h,
+      have x ∈ FV (t₁.to_termctx t') ∨ x ∈ FV (t₂.to_termctx t'), from free_in_prop.post.inv this,
+      or.elim this (
+        assume : x ∈ FV (t₁.to_termctx t'),
+        have x ∈ FV t₁, from free_in_termctx.term.inv this,
+        show x ∈ FV (prop.post t₁ t₂), from free_in_prop.post₁ this
+      ) (
+        assume : x ∈ FV (t₂.to_termctx t'),
+        have x ∈ FV t₂, from free_in_termctx.term.inv this,
+        show x ∈ FV (prop.post t₁ t₂), from free_in_prop.post₂ this
+      )
+    )},
+    case prop.call t₁ t₂ { from (
+      have prop.to_propctx (prop.call t₁ t₂) = propctx.call t₁ t₂, by unfold prop.to_propctx,
+      have h: x ∈ FV ((propctx.call t₁ t₂) t'), from this ▸ x_free_in_P,
+      have propctx.apply (propctx.call t₁.to_termctx t₂.to_termctx) t' = prop.call (t₁.to_termctx t') (t₂.to_termctx t'),
+      by unfold propctx.apply,
+      have x ∈ FV (prop.call (t₁.to_termctx t') (t₂.to_termctx t')), from this.symm ▸ h,
+      have x ∈ FV (t₁.to_termctx t') ∨ x ∈ FV (t₂.to_termctx t'), from free_in_prop.call.inv this,
+      or.elim this (
+        assume : x ∈ FV (t₁.to_termctx t'),
+        have x ∈ FV t₁, from free_in_termctx.term.inv this,
+        show x ∈ FV (prop.call t₁ t₂), from free_in_prop.call₁ this
+      ) (
+        assume : x ∈ FV (t₂.to_termctx t'),
+        have x ∈ FV t₂, from free_in_termctx.term.inv this,
+        show x ∈ FV (prop.call t₁ t₂), from free_in_prop.call₂ this
+      )
+    )},
+    case prop.forallc y t P₁ ih { from (
+      have prop.to_propctx (prop.forallc y t P₁) = propctx.forallc y t P₁.to_propctx, by unfold prop.to_propctx,
+      have h: x ∈ FV ((propctx.forallc y t.to_termctx P₁.to_propctx) t'), from this ▸ x_free_in_P,
+      have propctx.apply (propctx.forallc y t.to_termctx P₁.to_propctx) t'
+         = prop.forallc y (t.to_termctx t') (P₁.to_propctx.apply t'), by unfold propctx.apply,
+      have x ∈ FV (prop.forallc y (t.to_termctx t') (P₁.to_propctx.apply t')), from this.symm ▸ h,
+      have x_neq_y: x ≠ y, from (free_in_prop.forallc.inv this).left,
+      have x ∈ FV (t.to_termctx t') ∨ x ∈ FV (P₁.to_propctx.apply t'), from (free_in_prop.forallc.inv this).right,
+      or.elim this (
+        assume : x ∈ FV (t.to_termctx t'),
+        have x ∈ FV t, from free_in_termctx.term.inv this,
+        show x ∈ FV (prop.forallc y t P₁), from free_in_prop.forallc₁ x_neq_y this
+      ) (
+        assume : x ∈ FV (P₁.to_propctx.apply t'),
+        have x ∈ FV P₁, from ih this,
+        show x ∈ FV (prop.forallc y t P₁), from free_in_prop.forallc₂ x_neq_y this
+      )
+    )},
+    case prop.exis y P₁ ih { from (
+      have prop.to_propctx (prop.exis y P₁) = (propctx.exis y P₁.to_propctx), by unfold prop.to_propctx,
+      have h: x ∈ FV ((propctx.exis y P₁.to_propctx) t'), from this ▸ x_free_in_P,
+      have propctx.apply (propctx.exis y P₁.to_propctx) t' = prop.exis y (P₁.to_propctx.apply t'), by unfold propctx.apply,
+      have x ∈ FV (prop.exis y (P₁.to_propctx.apply t')), from this.symm ▸ h,
+      have x_neq_y: x ≠ y, from (free_in_prop.exis.inv this).left,
+      have x ∈ FV (P₁.to_propctx.apply t'), from (free_in_prop.exis.inv this).right,
+      have x ∈ FV P₁, from ih this,
+      show x ∈ FV (prop.exis y P₁), from free_in_prop.exis x_neq_y this
+    )}
+  end
+
+lemma free_in_propctx.term.inv {x: var} {t: termctx} {t': term}:
+      x ∈ FV ((propctx.term t) t') → x ∈ FV (t t') :=
+  assume x_free_in_t: x ∈ FV (propctx.apply (propctx.term t) t'),
+  have (propctx.apply (propctx.term t) t') = t t', by unfold propctx.apply,
+  have x ∈ FV (prop.term (t t')), from this ▸ x_free_in_t,
+  show x ∈ FV (t t'), from free_in_prop.term.inv this
+
+lemma free_in_propctx.and.inv {x: var} {Q₁ Q₂: propctx} {t: term}:
+      x ∈ FV ((Q₁ && Q₂) t) → x ∈ FV (Q₁ t) ∨ x ∈ FV (Q₂ t) :=
+  assume x_free_in_Q12: x ∈ FV ((Q₁ && Q₂) t),
+  have (propctx.apply (propctx.and Q₁ Q₂) t) = Q₁.apply t && Q₂.apply t, by unfold propctx.apply,
+  have x ∈ FV (Q₁.apply t && Q₂.apply t), from this ▸ x_free_in_Q12,
+  show x ∈ FV (Q₁ t) ∨ x ∈ FV (Q₂ t), from free_in_prop.and.inv this
+
+lemma free_in_propctx.exis.inv {x fx: var} {Q: propctx} {t: term}:
+      x ∈ FV ((propctx.exis fx Q) t) → x ≠ fx ∧ x ∈ FV (Q t) :=
+  assume x_free_in_eQt: x ∈ FV ((propctx.exis fx Q) t),
+  have (propctx.apply (propctx.exis fx Q) t) = prop.exis fx (Q.apply t), by unfold propctx.apply,
+  have x ∈ FV (prop.exis fx (Q.apply t)), from this ▸ x_free_in_eQt,
+  show x ≠ fx ∧ x ∈ FV (Q t), from free_in_prop.exis.inv this
